theories/SLFWPsem.v
@@ -1,0 +1,391 @@
+(**
+
+Separation Logic Foundations
+
+Chapter: "WPsem".
+
+Author: Arthur Charguéraud.
+License: MIT.
+
+*)
+
+Set Implicit Arguments.
+From Sep Require Export SLFRules.
+
+Implicit Types f : var.
+Implicit Types b : bool.
+Implicit Types v : val.
+Implicit Types h : heap.
+Implicit Types P : Prop.
+Implicit Types H : hprop.
+Implicit Types Q : val->hprop.
+
+
+(* ####################################################### *)
+(** * The chapter in a rush *)
+
+(** This chapter introduces the notion of weakest precondition
+    for Separation Logic triples. *)
+
+
+(* ******************************************************* *)
+(** ** Notion of weakest precondition *)
+
+(** We next introduce a function [wp], called "weakest precondition".
+    Given a term [t] and a postcondition [Q], this function computes 
+    a heap predicate [wp t Q] such that [triple t H Q] holds if and
+    only if [wp t Q] is weaker than the precondition [H]. Formally: *)
+
+Parameter wp : trm -> (val->hprop) -> hprop.
+
+Parameter wp_equiv : forall t H Q,
+  (triple t H Q) <-> (H ==> wp t Q).
+
+(** The [wp t Q] is called "weakest precondition" for two reasons.
+    First, because it is a "valid precondition" for the term [t] 
+    and the postcondition [Q]: *)
+
+Lemma wp_pre : forall t Q,
+  triple t (wp t Q) Q.
+Proof using. intros. rewrite wp_equiv. applys himpl_refl. Qed.
+
+(** Second, because it is the "weakest" of all valid preconditions
+    for the term [t] and the postcondition [Q], in the sense that
+    any other valid precondition [H] entails [wp t Q]. *)
+
+Lemma wp_weakest : forall t H Q,
+  triple t H Q ->
+  H ==> wp t Q.
+Proof using. introv M. rewrite <- wp_equiv. applys M. Qed.
+
+(** As prove further in this chapter, it is possible to 
+    define a function [wp] satisfying [wp_equiv]. Formally: *)
+
+Definition wp_characterization (wp:trm->(val->hprop)->hprop) :=
+  forall t H Q, (triple t H Q) <-> (H ==> wp t Q).
+
+Parameter wp_characterization_exists : exists wp0,
+  wp_characterization wp0.
+
+(** In fact, there are several ways in which [wp] can be defined.
+    It turns out that all possible definitions are equivalent.
+    In other words, [wp_equiv] defines a unique function.
+    We next formally justify this fact. *)
+
+Lemma wp_characterization_unique : forall wp1 wp2,
+  wp_characterization wp1 ->
+  wp_characterization wp2 ->
+  wp1 = wp2.
+Proof using. 
+  asserts L: (forall t Q wp1 wp2,
+    wp_characterization wp1 ->
+    wp_characterization wp2 ->
+    wp1 t Q ==> wp2 t Q).
+  { introv M1 M2. unfolds wp_characterization.
+    rewrite <- M2. rewrite M1. applys himpl_refl. }
+  introv M1 M2. applys fun_ext_2. intros t Q.
+  applys himpl_antisym; applys L; auto.
+Qed.
+
+(** Thus, it really does not matter which definition of [wp] is
+    considered. Thereafter, we only exploit the characterization lemma
+    [wp_equiv], and never rely on the internal definition of [wp]. *)
+
+
+(* ******************************************************* *)
+(** ** Structural properties of weakest preconditions *)
+
+(** It is interesting to observe how the structural rules
+    can be applied on a judgment of the form [H ==> wp t Q].
+
+    At this stage, we'll make four important observations.
+
+    1. The extraction rules [triple_hexists] and [triple_hpure]
+       are not needed in a wp-style presentation, because they
+       are directly subsumed by basic lemmas on entailment.
+
+    2. The predicate [wp t Q] is covariant in [Q], just the same
+       way [triple t H Q] is covariant in [Q] (and contravariant 
+       in [H]).
+
+    3. The combined consequence-frame-htop rule for [triple]
+       has a counterpart for [wp]. This rule is, in effect,
+       the unique structural rule that is needed for [wp].
+       (All other structural rules are derivable from it.)
+
+    4. The ramified-frame rule for [triple] also has a
+       counterpart for [wp]. This ramified rule for [wp]
+       will play a crucial rule in the construction of
+       our function that computes weakest precondition. *)
+
+(* ------------------------------------------------------- *)
+(** *** 1. Extraction rules are no longer needed *)
+
+(** Recall the extraction rule for existentials: *)
+
+Parameter triple_hexists : forall t (A:Type) (J:A->hprop) Q,
+  (forall x, triple t (J x) Q) ->
+  triple t (\exists x, J x) Q.
+
+(** Replacing [triple t H Q] with [H ==> wp t Q] yields: *)
+
+Lemma triple_hexists_in_wp : forall t Q A (J:A->hprop),
+  (forall x, (J x ==> wp t Q)) ->
+  (\exists x, J x) ==> wp t Q.
+
+(** This implication is just a special case of the lemma
+    [himpl_hexists_l], which proves [(\exists x, J x) ==> H]
+    from [forall x, (J x ==> H)]. *)
+
+Proof using. introv M. applys himpl_hexists_l M. Qed.
+
+(** In other words, in the [wp] presentation, we don't need
+    a specific extraction rule for existentials, because the
+    extraction rule for entailment already does the job. *)
+
+(** Likewise for [triple_hpure], which enables extracting pure
+    facts from precondition: the rule [himpl_hstar_hpure_l] may be
+    used to prove [\[P] \* H1 ==> H2] from [\[P] -> H1 ==> H2]. *)
+
+
+(* ------------------------------------------------------- *)
+(** *** 2. Covariance of [wp] *)
+
+(** If we have [triple t H Q1] and [Q1 ===> Q2], then, by the
+    rule of consequence, we can derive [triple t H Q2]. 
+    In other words, [triple t H Q] is covariant in [Q].
+
+    In a similiar way [wp t Q] is covariant in [Q], as we state
+    and prove next. *)
+
+Lemma wp_conseq : forall t Q1 Q2,
+  Q1 ===> Q2 ->
+  wp t Q1 ==> wp t Q2.
+Proof using.
+  introv WQ.
+  rewrite <- wp_equiv. (* same as [applys wp_weakest]. *)
+  applys triple_conseq (wp t Q1) WQ.
+  { rewrite wp_equiv. auto. (* same as [applys wp_pre]. *) }
+  { applys himpl_refl. }
+Qed.
+
+
+(* ------------------------------------------------------- *)
+(** *** 3. Combined structural rule for [wp] *)
+
+(** Recall the combined consequence-frame-htop rule for [triple]. *)
+
+Parameter triple_conseq_frame_htop : forall H2 H1 Q1 t H Q,
+  triple t H1 Q1 ->
+  H ==> H1 \* H2 ->
+  Q1 \*+ H2 ===> Q \*+ \Top ->
+  triple t H Q.
+
+(** Let us reformulate this rule using [wp]:
+
+[[
+    H1 ==> wp t Q1 ->
+    H ==> H1 \* H2 ->
+    Q1 \*+ H2 ===> Q \*+ \Top ->
+    H ==> wp t Q.
+]]
+
+   The beove statement can be simplified by substituting [H]
+   with [H1 \* H2], then substituting [H1] with [wp t Q1].
+   We obtain:
+
+[[
+    Q1 \*+ H2 ===> Q \*+ \Top ->
+    (wp t Q1) \* H2 ==> wp t Q.
+]]
+   After renaming [H2] into [H] and [Q] into [Q2], we arrive at
+   the combined rule for [wp]:
+*)
+
+Lemma wp_conseq_frame_htop : forall t H Q1 Q2,
+  Q1 \*+ H ===> Q2 \*+ \Top ->
+  (wp t Q1) \* H ==> (wp t Q2).
+Proof using.
+  introv M. rewrite <- wp_equiv.
+  applys triple_conseq_frame_htop (wp t Q1) M.
+  { rewrite wp_equiv. hsimpl. } { hsimpl. }
+Qed.
+
+(** Further in this chapter, we present specializations of
+    this rule to invoke only the [frame] rule, or only the
+    garbage collection rule. *)
+
+
+(* ------------------------------------------------------- *)
+(** *** 4. The ramified structural rule for [wp] *)
+
+(** Consider the entailment  [Q1 \*+ H ===> Q2 \*+ \Top]
+    that appears in the combined rule [wp_conseq_frame_htop].
+
+    This entailement can be rewritten using the magic wand as:
+    [H ==> (Q1 \--* (Q2 \*+ \Top))].
+
+    Thus, the conclusion [(wp t Q1) \* H ==> (wp t Q2)]
+    can be reformulated as 
+    [(wp t Q1) \* (Q1 \--* (Q2 \*+ \Top)) ==> (wp t Q2)].
+
+    The "ramified combined structural rule" for [wp], shown below,
+    captures in a single line all the structural properties of [wp]. *)
+
+Lemma wp_ramified : forall t Q1 Q2,
+  (wp t Q1) \* (Q1 \--* Q2 \*+ \Top) ==> (wp t Q2).
+Proof using.
+  intros. applys wp_conseq_frame_htop.
+  hsimpl. (* exploiting [qwand_cancel] *)
+Qed.
+
+(** The following reformulation is handy to apply on any goal
+    of the form [H ==> wp t Q]. *)
+
+Lemma wp_ramified_trans : forall t H Q1 Q2,
+  H ==> (wp t Q1) \* (Q1 \--* Q2 \*+ \Top) ->
+  H ==> (wp t Q2).
+Proof using. introv M. hchange M. applys wp_ramified. Qed.
+
+
+
+(* ####################################################### *)
+(** * Additional contents *)
+
+(* ******************************************************* *)
+(** ** Semantic definition of weakest precondition *)
+
+(** We have seen that [wp_equiv] defines a unique function [wp].
+    There remains to show that there actually exists at least
+    one such function.
+
+    In what follows, we'll give two possible definitions, a
+    low-level one expressed as a function on heaps, and a high-level
+    one expressed using only Separation Logic combinators.
+
+    For both, we'll show that they satisfy [wp_equiv]. Thus, the
+    two definitions must be equivalent ([wp_characterization_unique]). *)
+
+(** We now present the low-level definition. *)
+
+Definition wp_low (t:trm) (Q:val->hprop) : hprop :=
+  fun (h:heap) => triple t (=h) Q.
+
+Lemma wp_equiv_wp_low : wp_characterization wp_low.
+  (** [forall t H Q, (triple t H Q) <-> (H ==> wp_low t Q)]. *)
+Proof using.
+  (** This proof is a bit technical, it is not required to follow it.
+      It requires the lemma [triple_named_heap] established 
+      as exercise in an earlier chapter. *)
+  unfold wp_low. iff M.
+  { intros h K. applys triple_conseq M.
+    { intros h' ->. applys K. }
+    { applys qimpl_refl. } }
+  { applys triple_named_heap. intros h K.
+    applys triple_conseq (=h) Q. 
+    { specializes M K. applys M. }
+    { intros ? ->. auto. }
+    { applys qimpl_refl. } }
+Qed.
+
+(** We now present the high-level definition. *)
+
+Definition wp_high (t:trm) (Q:val->hprop) : hprop :=
+  \exists (H:hprop), H \* \[triple t H Q].
+
+(* EX3! (wp_equiv_wp_high) *)
+(** Prove that this second definition of [wp] statisfies
+    the characteristic property [wp_equiv]. *)
+
+Lemma wp_equiv_wp_high : wp_characterization wp_high.
+  (** [forall t H Q, (triple t H Q) <-> (H ==> wp_high t Q)]. *)
+Proof using.
+(* SOLUTION *)
+  unfold wp_characterization, wp_high. iff M.
+  { hsimpl H. apply M. }
+  { applys triple_conseq Q M.
+    { applys triple_hexists. intros H'.
+      rewrite hstar_comm. applys triple_hpure. 
+      intros N. applys N. }
+    { applys qimpl_refl. } }
+(* /SOLUTION *)
+Qed.
+
+
+(* ******************************************************* *)
+(** ** Frame rule and garbage rules for [wp] *)
+
+(** The combined structural rule for [wp] captures all the
+    structural rules. We here discuss the formulation of
+    specializations of this rule. The corresponding lemmas
+    highlight interesting properties of the [wp] operator. *)
+
+(** Recall the [wp_conseq] rule. *)
+
+Parameter wp_conseq' : forall t Q1 Q2,
+  Q1 ===> Q2 ->
+  wp t Q1 ==> wp t Q2.
+
+(** How can this rule simulate the rule of consequence, which also
+    enables strenthening the precondition? The following lemma
+    provides the answer: strenghtening of the precondition simply
+    consists of invoking the transitivy property of entailment. *)
+
+Lemma wp_conseq_pre : forall t H' H Q,
+  H' ==> wp t Q ->
+  H ==> H' ->
+  H ==> wp t Q.
+Proof using. introv M WH. applys himpl_trans WH. applys M. Qed.
+
+(** More generally, the consequence rule for goals in [wp] form
+    takes the form: *)
+
+Lemma wp_conseq_trans : forall t H' Q' H Q,
+  H' ==> wp t Q' ->
+  H ==> H' ->
+  Q' ===> Q ->
+  H ==> wp t Q.
+Proof using. introv M WH WQ. hchange WH. hchange M. applys wp_conseq WQ. Qed.
+
+(** Thereafter, we present rules in the form of entailments between [wp],
+    that is, [wp ... ==> wp ...], but keep in mind that this presentation
+    is equivalent to the form: [forall H, H ==> wp ... -> H ==> wp ...]. *)
+
+(** The frame rule for [wp] asserts that, given [(wp t Q) \* H],
+    the [wp] may absorb [H] and yield [(wp t (Q \*+ H)]. *)
+
+Lemma wp_frame : forall t H Q,
+  (wp t Q) \* H ==> wp t (Q \*+ H).
+Proof using.
+  intros. rewrite <- wp_equiv.
+  applys triple_frame. rewrite~ wp_equiv.
+Qed.
+
+(** The garbage collection in precondition for [wp] asserts that
+    [wp] can absorb and discard any desired heap predicate [H]
+    that sits next to it (i.e., that it is starred with). *)
+
+Lemma wp_hany_pre : forall t H Q,
+  (wp t Q) \* H ==> wp t Q.
+Proof using.
+  intros. rewrite <- wp_equiv.
+  applys triple_hany_pre. rewrite~ wp_equiv.
+Qed.
+
+(** The garbage collection in postconditions for [wp] asserts 
+    that [wp] can absorb and discard any desired heap predicate
+    [H] that appears in its postcondition. *)
+
+Lemma wp_hany_post : forall t H Q ,
+  wp t (Q \*+ H) ==> wp t Q.
+Proof using.
+  intros. rewrite <- wp_equiv.
+  applys triple_hany_post. rewrite~ wp_equiv.
+Qed.
+
+(** Note, equivalently, the [H] from rules [wp_hany_pre] and 
+   [wp_hand_post] may be replaced with [\Top]. *)
+
+
+
+
